src/cddl/pulse/CDDL.Pulse.Serialize.Base.fst
@@ -97,6 +97,40 @@ fn impl_serialize_ext
 }
 
 inline_for_extraction noextract [@@noextract_to "krml"]
+fn impl_serialize_bij
+    (#[@@@erasable]t: Ghost.erased typ)
+    (#[@@@erasable]tgt: Type0)
+    (#[@@@erasable] inj: Ghost.erased bool)
+    (#[@@@erasable]ps: Ghost.erased (spec t tgt inj))
+    (#impl_tgt: Type0)
+    (#[@@@erasable]r: rel impl_tgt tgt)
+    (i: impl_serialize ps r)
+    (#[@@@erasable]tgt' : Type0)
+    ([@@@erasable]f12: Ghost.erased (tgt -> tgt'))
+    ([@@@erasable]f21: Ghost.erased (tgt' -> tgt))
+    ([@@@erasable]fprf_21_12: (x: tgt) -> squash (Ghost.reveal f21 (Ghost.reveal f12 x) == x))
+    ([@@@erasable]fprf_12_21: (x: tgt') -> squash (Ghost.reveal f12 (Ghost.reveal f21 x) == x))
+    (#impl_tgt' : Type0)
+    (g12: (impl_tgt -> impl_tgt'))
+    (g21: (impl_tgt' -> impl_tgt))
+    ([@@@erasable]gprf_21_12: (x: impl_tgt) -> squash (g21 (g12 x) == x))
+    ([@@@erasable]gprf_12_21: (x: impl_tgt') -> squash (g12 (g21 x) == x))
+: impl_serialize #t #tgt' #inj (spec_inj ps f12 f21 fprf_21_12 fprf_12_21) #impl_tgt' (rel_fun r g21 f21)
+=
+    (c: _)
+    (#v: _)
+    (out: _)
+{
+  let c' = g21 c;
+  Trade.rewrite_with_trade
+    (rel_fun r g21 f21 c v)
+    (r c' (Ghost.reveal f21 v));
+  let res = i c' #(Ghost.reveal f21 v) out; // FIXME: WHY WHY WHY the explicit here?
+  Trade.elim _ _;
+  res
+}
+
+inline_for_extraction noextract [@@noextract_to "krml"]
 fn impl_serialize_choice
     (#[@@@erasable]t1: Ghost.erased typ)
     (#[@@@erasable]tgt1: Type0)
